Refactor: merge concrete and width-generic InstCombine dialects

SSA/Projects/InstCombine/Base.lean
@@ -1,109 +1,158 @@
 --import SSA.Core.WellTypedFramework
 import SSA.Experimental.IntrinsicAsymptotics
 import SSA.Core.Util
+import SSA.Core.Util.ConcreteOrMVar
 import SSA.Projects.InstCombine.ForMathlib
 
+/-!
+  # InstCombine Dialect
+
+  This file defines a dialect of basic arithmetic and bitwise operations on bitvectors.
+
+  The dialect supports types of arbitrary-width bitvectors.
+  Thus, some definitions wil be parameterized by `φ`, the number of width meta-variables there are.
+  This parameter will usually be either `0`, indicating that all widths are known, concrete values,
+  or `1`, indicating there is exactly one distinct width meta-variable.
+
+  In particular, we only define a denotational semantics for concrete programs (i.e., where `φ = 0`)
+  
+
+  see https://releases.llvm.org/14.0.0/docs/LangRef.html#bitwise-binary-operations
+-/
 
 namespace InstCombine
 
+abbrev Width φ := ConcreteOrMVar Nat φ
+
 inductive IntPredicate where
-| eq
-| ne
-| ugt
-| uge
-| ult
-| ule
-| sgt
-| sge
-| slt
-| sle
+  | eq
+  | ne
+  | ugt
+  | uge
+  | ult
+  | ule
+  | sgt
+  | sge
+  | slt
+  | sle
 deriving Inhabited, DecidableEq, Repr
 
-inductive Ty
-  | bitvec (w : Nat) : Ty
-  deriving DecidableEq, Inhabited, Repr
+inductive MTy (φ : Nat)
+  | bitvec (w : Width φ) : MTy φ
+  deriving DecidableEq, Inhabited
 
-instance : ToString Ty where
+abbrev Ty := MTy 0
+
+instance : Repr (MTy φ) where 
+  reprPrec 
+    | .bitvec (.concrete w), _ => "i" ++ repr w
+    | .bitvec (.mvar ⟨i, _⟩), _ => f!"i$\{%{i}}"
+
+instance : ToString (MTy φ) where
   toString t := repr t |>.pretty
 
-instance : Repr Ty where 
-  reprPrec 
-    | .bitvec w, _ => "i" ++ repr w
-
-instance {w : Nat} : Inhabited Ty := ⟨Ty.bitvec w⟩
-
 def Ty.width : Ty → Nat
-  | .bitvec w => w
+  | .bitvec (.concrete w) => w
 
 @[simp]
-theorem Ty.width_eq (ty : Ty) :  Ty.bitvec (ty.width) = ty :=
- by simp [width]
+theorem Ty.width_eq (ty : Ty) : .bitvec (ty.width) = ty := by 
+  rcases ty with ⟨w|i⟩
+  · rfl
+  · exact i.elim0
 
 @[simp]
 def Bitvec.width {n : Nat} (_ : Bitvec n) : Nat := n
 
 instance : Goedel Ty where
 toType := fun
-  | .bitvec w => Option $ Bitvec w
+  | .bitvec (.concrete w) => Option $ Bitvec w
 
 instance : Repr (Bitvec n) where
   reprPrec
     | v, n => reprPrec (Bitvec.toInt v) n
 
 -- See: https://releases.llvm.org/14.0.0/docs/LangRef.html#bitwise-binary-operations
-inductive Op
-| and (w : Nat) : Op
-| or (w : Nat) : Op
-| not (w : Nat) : Op
-| xor (w : Nat) : Op
-| shl (w : Nat) : Op
-| lshr (w : Nat) : Op
-| ashr (w : Nat) : Op
-| urem (w : Nat) : Op
-| srem (w : Nat) : Op
-| select (w : Nat) : Op
-| add (w : Nat) : Op
-| mul (w : Nat) : Op
-| sub (w : Nat) : Op
-| neg (w: Nat) : Op
-| copy (w: Nat) : Op
-| sdiv (w : Nat) : Op
-| udiv (w : Nat) : Op
-| icmp (c : IntPredicate) (w : Nat) : Op
-| const {w : Nat} (val : Bitvec w) : Op
+inductive MOp (φ : Nat) : Type
+  | and     (w : Width φ) : MOp φ
+  | or      (w : Width φ) : MOp φ
+  | not     (w : Width φ) : MOp φ
+  | xor     (w : Width φ) : MOp φ
+  | shl     (w : Width φ) : MOp φ
+  | lshr    (w : Width φ) : MOp φ
+  | ashr    (w : Width φ) : MOp φ
+  | urem    (w : Width φ) : MOp φ
+  | srem    (w : Width φ) : MOp φ
+  | select  (w : Width φ) : MOp φ
+  | add     (w : Width φ) : MOp φ
+  | mul     (w : Width φ) : MOp φ
+  | sub     (w : Width φ) : MOp φ
+  | neg     (w : Width φ) : MOp φ
+  | copy    (w : Width φ) : MOp φ
+  | sdiv    (w : Width φ) : MOp φ
+  | udiv    (w : Width φ) : MOp φ
+  | icmp    (c : IntPredicate) (w : Width φ) : MOp φ
+  /-- Since the width of the const might not be known, we just store the value as an `Int` -/
+  | const (w : Width φ) (val : ℤ) : MOp φ
 deriving Repr, DecidableEq, Inhabited
+
+abbrev Op := MOp 0
+
+namespace Op
+
+@[match_pattern] abbrev and    : Nat → Op := MOp.and    ∘ .concrete
+@[match_pattern] abbrev or     : Nat → Op := MOp.or     ∘ .concrete
+@[match_pattern] abbrev not    : Nat → Op := MOp.not    ∘ .concrete
+@[match_pattern] abbrev xor    : Nat → Op := MOp.xor    ∘ .concrete
+@[match_pattern] abbrev shl    : Nat → Op := MOp.shl    ∘ .concrete
+@[match_pattern] abbrev lshr   : Nat → Op := MOp.lshr   ∘ .concrete
+@[match_pattern] abbrev ashr   : Nat → Op := MOp.ashr   ∘ .concrete
+@[match_pattern] abbrev urem   : Nat → Op := MOp.urem   ∘ .concrete
+@[match_pattern] abbrev srem   : Nat → Op := MOp.srem   ∘ .concrete
+@[match_pattern] abbrev select : Nat → Op := MOp.select ∘ .concrete
+@[match_pattern] abbrev add    : Nat → Op := MOp.add    ∘ .concrete
+@[match_pattern] abbrev mul    : Nat → Op := MOp.mul    ∘ .concrete
+@[match_pattern] abbrev sub    : Nat → Op := MOp.sub    ∘ .concrete
+@[match_pattern] abbrev neg    : Nat → Op := MOp.neg    ∘ .concrete
+@[match_pattern] abbrev copy   : Nat → Op := MOp.copy   ∘ .concrete
+@[match_pattern] abbrev sdiv   : Nat → Op := MOp.sdiv   ∘ .concrete
+@[match_pattern] abbrev udiv   : Nat → Op := MOp.udiv   ∘ .concrete
+
+@[match_pattern] abbrev icmp (c : IntPredicate)   : Nat → Op  := MOp.icmp c ∘ .concrete
+@[match_pattern] abbrev const (w : Nat) (val : ℤ) : Op        := MOp.const (.concrete w) val
+
+end Op
 
 instance : ToString Op where
   toString o := repr o |>.pretty
 
 @[simp, reducible]
-def Op.sig : Op → List Ty
-| Op.and w | Op.or w | Op.xor w | Op.shl w | Op.lshr w | Op.ashr w
-| Op.add w | Op.mul w | Op.sub w | Op.udiv w | Op.sdiv w 
-| Op.srem w | Op.urem w | Op.icmp _ w =>
-  [Ty.bitvec w, Ty.bitvec w]
-| Op.not w | Op.neg w | Op.copy w => [Ty.bitvec w]
-| Op.select w => [Ty.bitvec 1, Ty.bitvec w, Ty.bitvec w]
-| Op.const _ => []
+def MOp.sig : MOp φ → List (MTy φ)
+| .and w | .or w | .xor w | .shl w | .lshr w | .ashr w
+| .add w | .mul w | .sub w | .udiv w | .sdiv w 
+| .srem w | .urem w | .icmp _ w =>
+  [.bitvec w, .bitvec w]
+| .not w | .neg w | .copy w => [.bitvec w]
+| .select w => [.bitvec 1, .bitvec w, .bitvec w]
+| .const _ _ => []
 
 @[simp, reducible]
-def Op.outTy : Op → Ty
-| Op.and w | Op.or w | Op.not w | Op.xor w | Op.shl w | Op.lshr w | Op.ashr w
-| Op.sub w |  Op.select w | Op.neg w | Op.copy w =>
-  Ty.bitvec w
-| Op.add w | Op.mul w |  Op.sdiv w | Op.udiv w | Op.srem w | Op.urem w =>
-  Ty.bitvec w
-| Op.icmp _ _ => Ty.bitvec 1
-| @Op.const width _ => Ty.bitvec width
+def MOp.outTy : MOp φ → MTy φ
+| .and w | .or w | .not w | .xor w | .shl w | .lshr w | .ashr w
+| .sub w |  .select w | .neg w | .copy w =>
+  .bitvec w
+| .add w | .mul w |  .sdiv w | .udiv w | .srem w | .urem w =>
+  .bitvec w
+| .icmp _ _ => .bitvec 1
+| .const width _ => .bitvec width
 
-instance : OpSignature Op Ty where 
+instance : OpSignature (MOp φ) (MTy φ) where 
   signature op := ⟨op.sig, [], op.outTy⟩
 
 @[simp]
 def Op.denote (o : Op) (arg : HVector Goedel.toType (OpSignature.sig o)) :
     (Goedel.toType <| OpSignature.outTy o) :=
   match o with
-  | Op.const c => Option.some c
+  | Op.const w val => Option.some (Bitvec.ofInt w val)
   | Op.and _ => pairMapM (.&&&.) arg.toPair
   | Op.or _ => pairMapM (.|||.) arg.toPair
   | Op.xor _ => pairMapM (.^^^.) arg.toPair
