SSA/Core/Util/ConcreteOrMVar.lean
@@ -1,0 +1,45 @@
+import Mathlib.Data.Fin.Basic
+import Mathlib.Data.Vector.Basic
+-- import Mathlib.Tactic
+
+
+/-- 
+  A general type that is either a concrete known value of type `α`, or one of `φ` metavariables
+ -/
+inductive ConcreteOrMVar (α : Type u) (φ : Nat)
+  | concrete (a : α)
+  | mvar (i : Fin φ)
+  deriving DecidableEq, Repr, Inhabited
+
+/-- A coercion from the concrete type `α` to the `ConcreteOrMVar` -/
+instance : Coe α (ConcreteOrMVar α φ) := ⟨.concrete⟩
+
+/- In the specific case of `α := Nat`, we'd like to be able to use nat literals -/
+instance : OfNat (ConcreteOrMVar Nat φ) n := ⟨.concrete n⟩
+
+namespace ConcreteOrMVar 
+
+/-- If there are no meta-variables, `ConcreteOrMVar` is just the concrete type `α` -/
+def toConcrete : ConcreteOrMVar α 0 → α 
+  | .concrete a => a
+
+@[simp]
+theorem toConcrete_concrete : toConcrete (.concrete a) = a := rfl
+
+/-- 
+  Provide a value for one of the metavariables.
+  Specifically, the metavariable with the maximal index `φ` out of `φ+1` total metavariables.
+  All other metavariables indices' are left as-is, but cast to `Fin φ` -/
+def instantiateOne (a : α) : ConcreteOrMVar α (φ+1) → ConcreteOrMVar α φ
+  | .concrete w => .concrete w
+  | .mvar i => i.lastCases 
+      (.concrete a)       -- `i = Fin.last`
+      (fun j => .mvar j)  -- `i = Fin.castSucc j`
+
+/-- Instantiate all meta-variables -/
+def instantiate (as : Vector α φ) : ConcreteOrMVar α φ → α
+  | .concrete w => w
+  | .mvar i => as.get i
+
+
+end ConcreteOrMVar
